Fix up enum, finally!

ha2_enum.v
@@ -1,744 +1,605 @@
-Require Import ha2_refl.
+Require Import ha2_refl countable.
 Close Scope subst_scope.
 Require Import List.
 
 Import ListNotations.
 
-Fixpoint vars_up_to (n : nat) : list fin :=
-  match n with
-  | 0 => [0]
-  | S m => n :: vars_up_to m
+Check [0].
+Check [0; 1; 2; 3].
+
+Check @enum_iso.
+Print retract.
+
+Print gen_tree.
+Print tm.
+Locate tm.
+
+Fixpoint tm_to_gen_tree (t : tm) : gen_tree fin :=
+  match t with
+  | var_tm x => gen_cons 0 ([gen_nil x])
+  | Z => gen_cons 1 ([])
+  | Succ t => gen_cons 2 ([tm_to_gen_tree t])
+  | ha2_syn.Add t1 t2 => gen_cons 3 ([tm_to_gen_tree t1; tm_to_gen_tree t2])
+  | Mult t1 t2 => gen_cons 4 ([tm_to_gen_tree t1; tm_to_gen_tree t2])
   end.
 
+Search (_ -> _ -> option _).
 
-Class has_depth A := { depth : A -> nat }.
+Definition bind_opt {A B} (o : option A) (f : A -> option B) : option B :=
+  match o with
+  | Datatypes.Some a => f a
+  | Datatypes.None => @Datatypes.None B
+  end.
 
-Instance has_depth_fin : has_depth fin := {| depth n := n |}.
+Definition map_opt {A B} (o : option A) (f : A -> B) : option B :=
+  match o with
+  | Datatypes.Some a => Some (f a)
+  | Datatypes.None => @Datatypes.None B
+  end.
 
-(* Let's see if we need this... *)
-Class enum A {d : has_depth A} :=
-  {
-    list_up_to : nat -> list A;
-    list_has_all : forall n (a : A), depth a <= n -> In a (list_up_to n);
-  }.
+Definition map_opt_2 {A B C} (o1 : option A) (o2 : option B) (f : A -> B -> C) : option C :=
+  match (pair o1 o2) with
+  | pair (Datatypes.Some a) (Datatypes.Some b) => Some (f a b)
+  | _ => None
+  end.
 
-(* Useful if we're defining the set of elements of depth less than n by induction *)
-Class enum_up_to A {d : has_depth A} n :=
-  {
-    list_le_n : list A;
-    list_has_all_n : forall a, depth a <= n -> In a list_le_n;
-  }.
+Fixpoint gen_tree_to_tm (g : gen_tree fin) : option tm :=
+  match g with
+  | gen_cons 0 ([gen_nil x]) => Some (var_tm x)
+  | gen_cons 1 ([]) => Some Z
+  | gen_cons 2 ([g']) => map_opt (gen_tree_to_tm g') Succ
+  | gen_cons 3 ([g1; g2]) => map_opt_2 (gen_tree_to_tm g1) (gen_tree_to_tm g2) ha2_syn.Add
+  | gen_cons 4 ([g1; g2]) => map_opt_2 (gen_tree_to_tm g1) (gen_tree_to_tm g2) Mult
+  | _ => None
+  end.
 
-Instance enum_up_to_enum {A} {d : has_depth A} (h : forall n, enum_up_to A n) : enum A.
+Print retract.
+
+Definition retract_tm : retract (gen_tree fin) tm.
 Proof.
-  refine {| list_up_to := fun n => @list_le_n _ _ _ (h n) |}.
-  intros.
-  destruct (h n); simpl.
+  refine {| in_A := tm_to_gen_tree; out_A := gen_tree_to_tm |}.
+  induction b; simpl; auto.
+  - rewrite IHb; auto.
+  - rewrite IHb1, IHb2; auto.
+  - rewrite IHb1, IHb2; auto.
+Defined.
+
+Check @has_depth_iso.
+
+
+Instance has_depth_tm : has_depth tm.
+Proof.
+  apply (has_depth_iso retract_tm).
+Defined.
+
+Instance enum_tm : enum tm.
+Proof.
+  apply enum_iso.
+Defined.
+
+Print enum.
+
+Eval vm_compute in list_up_to 4 : list tm.
+
+(* Ok let's see if we can do propositions *)
+Print gen_tree.
+Print prop.
+
+Fixpoint prop_to_gen_tree (p : prop) : gen_tree (tm + fin) :=
+  match p with
+  | t ∈ pr => gen_cons 0 ([gen_nil (inl t); pred_to_gen_tree pr])
+  | all p' => gen_cons 1 ([prop_to_gen_tree p'])
+  | FORALL p' => gen_cons 2 ([prop_to_gen_tree p'])
+  | p1 ⇒ p2 => gen_cons 3 ([prop_to_gen_tree p1; prop_to_gen_tree p2])
+  end
+  with pred_to_gen_tree (pr : pred) : gen_tree (tm + fin) :=
+    match pr with
+    | var_pred v => gen_nil (inr v)
+    | {{ _ | p }} => gen_cons 4 ([prop_to_gen_tree p])
+    end.
+
+Fixpoint gen_tree_to_prop (g : gen_tree (tm + fin)) : option prop :=
+  match g with
+  | gen_cons 0 ([gen_nil (inl t); g']) =>
+      let pr := gen_tree_to_pred g' in
+      map_opt pr (fun pr => t ∈ pr)
+  | gen_cons 1 ([g']) =>
+      map_opt (gen_tree_to_prop g') (fun p => all p)
+  | gen_cons 2 ([g']) =>
+      map_opt (gen_tree_to_prop g') (fun p => FORALL p)
+  | gen_cons 3 ([g1; g2]) =>
+      let p1 := gen_tree_to_prop g1 in
+      let p2 := gen_tree_to_prop g2 in
+      map_opt_2 p1 p2 (fun p1 p2 => p1 ⇒ p2)
+  | _ => None
+  end
+with gen_tree_to_pred (g : gen_tree (tm + fin)) : option pred :=
+       match g with
+       | gen_nil (inr v) => Some (var_pred v)
+       | gen_cons 4 ([g]) =>
+           map_opt (gen_tree_to_prop g) (fun p => {{ _ | p }})
+       | _ => None
+  end
+.
+
+Print Instances enum.
+
+Definition retract_prop : retract (gen_tree (tm + fin)) prop.
+Proof.
+  refine {|
+      in_A := prop_to_gen_tree;
+      out_A := gen_tree_to_prop;
+    |}.
+  intros P.
+  induction P using prop_pred_ind with
+    (P0 := fun p => gen_tree_to_pred (pred_to_gen_tree p) = Datatypes.Some p);
+    simpl; try rewrite IHP; simpl; auto.
+  rewrite IHP1, IHP2.
+  unfold map_opt_2.
   auto.
 Defined.
 
-Instance enum_enum_up_to {A} {d : has_depth A} {e : enum A} : forall n, enum_up_to A n.
+Definition retract_pred : retract (gen_tree (tm + fin)) pred.
 Proof.
-  intro n.
-  refine {| list_le_n := list_up_to n |}.
-  destruct e; auto.
+  refine {|
+      in_A := pred_to_gen_tree;
+      out_A := gen_tree_to_pred;
+    |}.
+  intros P.
+  induction P; simpl; auto.
+  unfold map_opt.
+  Print retract.
+  pose (r := (@is_gen_retract _ _ retract_prop)).
+  simpl in r.
+  rewrite r.
+  auto.
 Defined.
+
+Goal enum (tm + fin).
+  apply _.
+Qed.
+
+Instance has_depth_prop : has_depth prop.
+Proof.
+  eapply @has_depth_iso; eauto.
+  - apply (_ : has_depth (gen_tree (tm + fin))).
+  - apply retract_prop.
+Defined.
+
+Instance has_depth_pred : has_depth pred.
+Proof.
+  eapply @has_depth_iso; eauto.
+  - apply (_ : has_depth (gen_tree (tm + fin))).
+  - apply retract_pred.
+Defined.
+
+Instance enum_prop : enum prop.
+Proof.
+  apply enum_iso.
+Defined.
+
+Check @list_up_to.
+
+Eval compute in depth (FORALL all var_tm 0 ∈ var_pred 0).
+
+Eval vm_compute in (list_up_to 3: list (gen_tree (fin + tm))).
+
+Eval vm_compute in (list_up_to 3: list prop).
+
+Print derives.
+
+Print Instances enum.
+
+Instance enum_ctxt : enum ctxt.
+Proof. apply _. Defined.
+
+Inductive derivation_leaf :=
+| Loc : nat -> derivation_leaf
+| Ctxt : ctxt -> derivation_leaf
+| PropLeaf : prop -> derivation_leaf
+| Pred : pred -> derivation_leaf
+| Tm : tm -> derivation_leaf.
+
+Fixpoint derives_to_gen_tree {Γ P} (d : Γ ⊢ P) : gen_tree derivation_leaf :=
+  match d with
+  | axiom n Γ P _ => gen_cons 0 ([
+                                    gen_nil (Loc n);
+                                    gen_nil (Ctxt Γ)
+                                ])
+  | imp_intro Γ P Q p => gen_cons 1 ([
+                                        gen_nil (Ctxt Γ);
+                                        gen_nil (PropLeaf P);
+                                        gen_nil (PropLeaf Q);
+                                        derives_to_gen_tree p
+                                    ])
+  | forallt_intro Γ P p => gen_cons 2 ([
+                                          gen_nil (Ctxt Γ);
+                                          gen_nil (PropLeaf P);
+                                          derives_to_gen_tree p
+                                      ])
+  | forallP_intro Γ P p => gen_cons 3 ([
+                                          gen_nil (Ctxt Γ);
+                                          gen_nil (PropLeaf P);
+                                          derives_to_gen_tree p
+                                      ])
+  | imp_elim Γ P Q p q => gen_cons 4 ([
+                                         gen_nil (Ctxt Γ);
+                                         gen_nil (PropLeaf P);
+                                         gen_nil (PropLeaf Q);
+                                         derives_to_gen_tree p;
+                                         derives_to_gen_tree q
+                                     ])
+  | forallt_elim Γ P t p => gen_cons 5 ([
+                                           gen_nil (Ctxt Γ);
+                                           gen_nil (PropLeaf P);
+                                           gen_nil (Tm t);
+                                           derives_to_gen_tree p
+                                       ])
+  | forallP_elim Γ P Q p => gen_cons 6 ([
+                                           gen_nil (Ctxt Γ);
+                                           gen_nil (PropLeaf P);
+                                           gen_nil (Pred Q);
+                                           derives_to_gen_tree p
+                                       ])
+  | compr_intro Γ P t p => gen_cons 7 ([
+                                          gen_nil (Ctxt Γ);
+                                          gen_nil (PropLeaf P);
+                                          gen_nil (Tm t);
+                                          derives_to_gen_tree p
+                                      ])
+  | compr_elim Γ P t p => gen_cons 8 ([
+                                         gen_nil (Ctxt Γ);
+                                         gen_nil (PropLeaf P);
+                                         gen_nil (Tm t);
+                                         derives_to_gen_tree p
+                                     ])
+  | zero_S Γ => gen_cons 9 ([gen_nil (Ctxt Γ)])
+  | inj_S Γ => gen_cons 10 ([gen_nil (Ctxt Γ)])
+  | plus_Z Γ => gen_cons 11 ([gen_nil (Ctxt Γ)])
+  | plus_S Γ => gen_cons 12 ([gen_nil (Ctxt Γ)])
+  | times_Z Γ => gen_cons 13 ([gen_nil (Ctxt Γ)])
+  | times_S Γ => gen_cons 14 ([gen_nil (Ctxt Γ)])
+  end.
+
+Lemma eqdec_tm : forall (t u : tm), {t = u} + {t <> u}.
+Proof.
+  decide equality.
+  decide equality.
+Qed.
+
+Lemma eqdec_prop : forall (p q : prop), {p = q} + {p <> q}
+with eqdec_pred : forall (p q : pred),  {p = q} + {p <> q}.
+Proof.
+  repeat decide equality.
+  repeat decide equality.
+Qed.
+
+Lemma eqdec_ctxt : forall (Γ Δ : ctxt), {Γ = Δ} + {Γ <> Δ}.
+Proof.
+  decide equality.
+  apply eqdec_prop.
+Qed.
+
+Hint Resolve eqdec_prop eqdec_ctxt eqdec_pred.
+
+Open Scope subst_scope.
+
+Lemma nth_error_dec (Γ : ctxt) n P : { nth_error Γ n = Some P } + { nth_error Γ n <> Some P}.
+Proof.
+  destruct (nth_error Γ n) eqn:eq; [ | right; intro h; inversion h].
+  destruct (eqdec_prop P p); [left | right].
+  - subst; auto.
+  - intro h; inversion h; subst; congruence.
+Qed.
+
+Require Import Coq.Logic.Eqdep_dec.
+
+
+Check UIP_dec.
+
+Lemma eqdec_refl : forall A (x : A) (p : { x = x } + { x <> x }), (forall (x y : A), {x = y} + {x <> y}) -> p = left Logic.eq_refl.
+Proof.
+  intros; destruct p.
+  - f_equal; apply UIP_dec; auto.
+  - congruence.
+Qed.
+
+Fixpoint gen_tree_to_derives (g : gen_tree derivation_leaf) Γ P : option (Γ ⊢ P).
+  refine
+    (match g with
+     | gen_cons 0 ([
+                      gen_nil (Loc n);
+                      gen_nil (Ctxt Γ)
+                  ]) => _
+     | gen_cons 1 ([
+                      gen_nil (Ctxt Γ);
+                      gen_nil (PropLeaf P);
+                      gen_nil (PropLeaf Q);
+                      p
+               ]) =>  _
+     | gen_cons 2 ([
+                      gen_nil (Ctxt Γ);
+                      gen_nil (PropLeaf P);
+                      p
+                  ]) =>  _
+     | gen_cons 3 ([
+                      gen_nil (Ctxt Γ);
+                      gen_nil (PropLeaf P);
+                      p
+                  ]) =>  _
+     | gen_cons 4 ([
+                      gen_nil (Ctxt Γ);
+                      gen_nil (PropLeaf P);
+                      gen_nil (PropLeaf Q);
+                      p;
+                      q
+               ]) =>  _
+     | gen_cons 5 ([
+                      gen_nil (Ctxt Γ);
+                      gen_nil (PropLeaf P);
+                      gen_nil (Tm t);
+                      p
+                  ]) => _
+     | gen_cons 6 ([
+                      gen_nil (Ctxt Γ);
+                      gen_nil (PropLeaf P);
+                      gen_nil (Pred Q);
+                      p
+                  ]) =>  _
+     | gen_cons 7 ([
+                      gen_nil (Ctxt Γ);
+                      gen_nil (PropLeaf P);
+                      gen_nil (Tm t);
+                      p
+                  ]) =>  _
+     | gen_cons 8 ([
+                      gen_nil (Ctxt Γ);
+                      gen_nil (PropLeaf P);
+                      gen_nil (Tm t);
+                      p
+                  ]) =>  _
+     | gen_cons 9 ([gen_nil (Ctxt Γ)]) => _
+     | gen_cons 10 ([gen_nil (Ctxt Γ)]) => _
+     | gen_cons 11 ([gen_nil (Ctxt Γ)]) => _
+     | gen_cons 12 ([gen_nil (Ctxt Γ)]) => _
+     | gen_cons 13 ([gen_nil (Ctxt Γ)]) => _
+     | gen_cons 14 ([gen_nil (Ctxt Γ)]) => _
+     | _ => None
+     end).
+  - destruct (nth_error_dec Γ n P); [| exact None].
+    destruct (eqdec_ctxt Γ0 Γ);
+      [ | exact None].
+    apply Some; subst; eapply axiom.
+    exact e.
+  - destruct (gen_tree_to_derives p (P::Γ) Q); [| exact None].
+    destruct (eqdec_ctxt Γ0  Γ); [ | exact None].
+    destruct (eqdec_prop P0 (P ⇒ Q)); [ | exact None].
+    subst.
+    apply Some; apply imp_intro; exact d2.
+  - destruct (gen_tree_to_derives p (lift_tm Γ) P); [ | exact None].
+    destruct (eqdec_ctxt Γ0 Γ); [ | exact None].
+    destruct (eqdec_prop P0 (all P)); [ | exact None].
+    subst; apply Some; eapply forallt_intro; exact d1.
+  - destruct (gen_tree_to_derives p (lift_prop Γ) P); [ | exact None].
+    destruct (eqdec_ctxt Γ0 Γ); [ | exact None].
+    destruct (eqdec_prop P0 (FORALL P)); [ | exact None].
+    subst; apply Some; eapply forallP_intro; exact d1.
+  - destruct (gen_tree_to_derives p Γ (P ⇒ Q)); [ | exact None].
+    destruct (gen_tree_to_derives q Γ P); [ | exact None].
+    destruct (eqdec_ctxt Γ0 Γ); [ | exact None].
+    destruct (eqdec_prop P0 Q); [| exact None].
+    subst; apply Some; eapply imp_elim; eauto.
+  - destruct (gen_tree_to_derives p Γ (all P)); [ | exact None].
+    destruct (eqdec_ctxt Γ0 Γ); [ | exact None].
+    destruct (eqdec_prop P0 (P[t..;ids])); [ | exact None].
+    subst.
+    apply Some.
+    apply forallt_elim.
+    exact d2.
+  - destruct (gen_tree_to_derives p Γ (FORALL P)); [ | exact None].
+    destruct (eqdec_ctxt Γ0 Γ); [ | exact None].
+    destruct (eqdec_prop P0 (P[ids;Q..])); [ | exact None].
+    subst.
+    apply Some.
+    apply forallP_elim.
+    exact d2.
+  - destruct (gen_tree_to_derives p Γ P[t..;ids]); [| exact None].
+    destruct (eqdec_ctxt Γ0 Γ); [ | exact None].
+    destruct (eqdec_prop P0 (t ∈ {{ _ | P }})); [ | exact None].
+    subst.
+    apply Some; eapply compr_intro.
+    exact d2.
+  - destruct (gen_tree_to_derives p Γ (t ∈ {{_ | P}})); [|exact None].
+    destruct (eqdec_ctxt Γ0 Γ); [| exact None].
+    destruct (eqdec_prop P0 P[t..; ids]); [|exact None].
+    subst; apply Some; eapply compr_elim.
+    exact d2.
+  - destruct (eqdec_ctxt Γ0 Γ); [|exact None].
+    destruct (eqdec_prop P (all Succ (var_tm 0) ≄ Z)); [|exact None].
+    subst; apply Some; apply zero_S.
+  - destruct (eqdec_ctxt Γ0 Γ); [|exact None].
+    destruct (eqdec_prop P (all all Succ (var_tm 1) ≃ Succ (var_tm 0) ⇒ var_tm 1 ≃ var_tm 0)); [|exact None].
+    subst; apply Some; apply inj_S.
+  - destruct (eqdec_ctxt Γ0 Γ); [|exact None].
+    destruct (eqdec_prop P (all ha2_syn.Add (var_tm 0) Z ≃ var_tm 0)); [|exact None].
+    subst; apply Some; apply plus_Z.
+  - destruct (eqdec_ctxt Γ0 Γ); [|exact None].
+    destruct (eqdec_prop P (all (all ha2_syn.Add (var_tm 1) (Succ (var_tm 0)) ≃ Succ (ha2_syn.Add (var_tm 1) (var_tm 0))))); [|exact None].
+    subst; apply Some; apply plus_S.
+  - destruct (eqdec_ctxt Γ0 Γ); [|exact None].
+    destruct (eqdec_prop P (all Mult (var_tm 0) Z ≃ Z)); [|exact None].
+    subst; apply Some; apply times_Z.
+  - destruct (eqdec_ctxt Γ0 Γ); [|exact None].
+    destruct (eqdec_prop P (all (all Mult (var_tm 1) (Succ (var_tm 0)) ≃ ha2_syn.Add (var_tm 1) (Mult (var_tm 1) (var_tm 0))))); [|exact None].
+    subst; apply Some; apply times_S.
+Defined.
+
+
+Ltac elim_eqdec :=
+  lazymatch goal with
+  | [ |- context[eqdec_ctxt ?X ?X] ] =>
+      assert (ee : eqdec_ctxt X X = left Logic.eq_refl) by (apply eqdec_refl; auto);
+      rewrite ee; clear ee; unfold eq_rec_r; simpl; auto
+  | [ |- context[eqdec_prop ?X ?X] ] =>
+      assert (ee : eqdec_prop X X = left Logic.eq_refl) by (apply eqdec_refl; auto);
+      rewrite ee; clear ee; unfold eq_rec_r; simpl; auto
+  | [ |- context[eqdec_tm ?X ?X] ] =>
+      assert (ee : eqdec_tm X X = left Logic.eq_refl) by (apply eqdec_refl; auto);
+      rewrite ee; clear ee; unfold eq_rec_r; simpl; auto
+  | _ => fail
+  end.
+
+Lemma is_retract_proof_to_gen_tree : forall Γ P (p : Γ ⊢ P),
+    gen_tree_to_derives (derives_to_gen_tree p) Γ P = Some p.
+Proof.
+  induction p; try (simpl; try rewrite IHp; simpl; now repeat elim_eqdec).
+  - simpl; destruct (nth_error_dec Γ n P).
+    + elim_eqdec.
+      f_equal; f_equal; auto.
+      apply UIP_dec; decide equality.
+    + subst; congruence.
+  - simpl; rewrite IHp1, IHp2; simpl.
+    repeat elim_eqdec.
+Qed.
+
+Print retract.
+
+Instance retract_derives Γ P : retract (gen_tree derivation_leaf) (Γ ⊢ P).
+Proof.
+  refine {| in_A := derives_to_gen_tree; out_A g := gen_tree_to_derives g Γ P |}.
+  apply is_retract_proof_to_gen_tree.
+Defined.
+
+
+Print derivation_leaf.
+
+Print Instances has_depth.
+
+Instance has_depth_derivation_leaf : has_depth derivation_leaf :=
+  {|
+    depth l :=
+    match l with
+    | Loc n => S n
+    | Ctxt Γ => depth Γ
+    | PropLeaf p => depth p
+    | Pred p => depth p
+    | Tm t => depth t
+    end
+  |}.
+
+Print enum.
+
+Instance enum_derivation_leaf : enum derivation_leaf.
+Proof.
+  refine
+    {|
+      list_up_to n :=
+      let locs := map Loc (list_up_to n) in
+      let ctxts := map Ctxt (list_up_to n) in
+      let props := map PropLeaf (list_up_to n) in
+      let preds := map Pred (list_up_to n) in
+      let tms := map Tm (list_up_to n) in
+      locs ++ ctxts ++ props ++ preds ++ tms
+    |}.
+  intros n a dpth; destruct a; simpl in dpth; repeat rewrite in_app_iff.
+  - left.
+    apply in_map.
+    apply list_has_all; auto.
+  - right; left.
+    apply in_map; apply list_has_all; auto.
+  - right; right; left.
+    apply in_map; apply list_has_all; auto.
+  - right; right; right; left;    
+    apply in_map; apply list_has_all; auto.
+  - right; right; right; right;
+      apply in_map; apply list_has_all; auto.
+Defined.
+
+Instance has_depth_derives Γ P : has_depth (Γ ⊢ P).
+Proof.
+  Check @has_depth_iso.
+  eapply @has_depth_iso.
+  apply (_ : has_depth (gen_tree derivation_leaf)).
+  apply retract_derives.
+Defined.
+
+Instance enum_derives Γ P : enum (Γ ⊢ P).
+Proof.
+  eapply @enum_iso.
+  apply _.
+Defined.
+
+
+(* TODO: define proof bundles and enum them. *)
+
+Record proof_bundle := { hyps : ctxt; concl : prop; proof : hyps ⊢ concl }.
+
+
+Print countable.has_depth.
+
+Instance has_depth_proof_bundle : has_depth proof_bundle :=
+  {|
+    depth b :=
+    let '{| hyps := hyps; concl := concl; proof:= proof |} := b in
+    depth hyps + depth concl + depth proof
+  |}.
+
+Print Instances enum.
+
+Check concat_map.
+Search (list (list _) -> _).
+
+Definition concat_map {A B} (f : A -> list B) l :=
+  concat (map f l).
+
+Lemma in_concat_map : forall A B (f : A -> list B) l x,
+    (exists y, In y l /\ In x (f y)) -> In x (concat_map f l).
+Proof.
+  intros.
+  apply in_concat.
+  destruct H as [y [in_y in_x]].
+  exists (f y); split; auto.
+  apply in_map; auto.
+Qed.
+
+Print enum.
 
 Require Import Lia.
 
-Instance enum_fin : enum fin.
-Proof.
-  refine {| list_up_to := vars_up_to |}.
-  induction n; simpl; intros; [ lia | ].
-  assert (h : a <= n \/ a = S n) by lia.
-  destruct h; [ | lia ].
-  right; auto.
-Defined.
-
-Generalizable Variable A.
-
-Fixpoint depth_list `{has_depth A} (l : list A) : nat :=
-  match l with
-  | [] => S 0
-  | a::aa => S (depth a + depth_list aa)
-  end.
-
-Definition apply_1 {A B} (f : A -> B)(l : list A) : list B := map f l.
-
-Lemma mem_apply_1 : forall {A B} (l : list A) (a : A) (f : A -> B),
-    In a l -> In (f a) (apply_1 f l).
-Proof.
-  Search map.
-  intros; apply in_map; auto.
-Qed.
-
-Fixpoint apply_2 {A B C} (f : A -> B -> C)(l1 : list A) (l2 : list B) : list C :=
-  match l1 with
-  | [] => []
-  | a::aa => (apply_1 (f a) l2) ++ apply_2 f aa l2
-  end.
-
-Lemma mem_apply_2 : forall {A B C} (l1 : list A) (l2 : list B) a b (f : A -> B -> C),
-    In a l1 -> In b l2 -> In (f a b) (apply_2 f l1 l2).
-Proof.
-  intros until l1.
-  induction l1; simpl; auto.
-  intros until f.
-  intros [h1 | h2] h; subst.
-  - apply in_or_app; left; apply mem_apply_1; auto.
-  - apply in_or_app; right; auto.
-Qed.
-
-Instance has_depth_pair {A B} {da : has_depth A} {db : has_depth B} : has_depth (A * B) := {| depth (p : A * B) := let (a, b) := p in depth a + depth b |}.
-
-Instance enum_pair {A B} `{ea : enum A} `{eb : enum B} : enum (A * B).
-refine {| list_up_to n := apply_2 (@pair A B) (list_up_to n) (list_up_to n) |}.
-destruct ea, eb.
-intros n [a b] h;
-  simpl in h.
-apply mem_apply_2; [apply list_has_all0; lia | apply list_has_all1; lia ].
-Defined.
-
-Record enum_component_1 B n :=
-  {
-    enum_ty :> Type;
-    constr : enum_ty -> B;
-    ha_depth_ty : has_depth enum_ty;
-    is_enum_ty : enum_up_to enum_ty n;
-  }.
-
-(* (* Since most of our constructors have *at most* 2 arguments, we *)
-(*    define a type that has exactly 2, and will put in dummy unit args *)
-(*    if they have fewer, and tuple them up if there are more. *)
-(* *) *)
-(* Record enum_component_2 C n := *)
-(*   { *)
-(*     enum_ty1 : Type; *)
-(*     enum_ty2 : Type; *)
-(*     constr : enum_ty1 -> enum_ty2 -> C; *)
-(*     has_depth_ty1 : has_depth enum_ty1; *)
-(*     has_depth_ty2 : has_depth enum_ty2; *)
-(*     is_enum_ty1 : enum_up_to enum_ty1 n; *)
-(*     is_enum_ty2 : enum_up_to enum_ty2 n; *)
-(*   }. *)
-
-
-(* Useful dummy instances *)
-Instance has_depth_false : has_depth False :=
-  {| depth (f : False) := match f with end |}.
-
-Instance enum_false : enum False.
-Proof.
-  refine {| list_up_to _ := [] |}.
-  intros; auto.
-Defined.
-
-Instance has_depth_tt : has_depth unit :=
-  {| depth (_ : unit) := 0 |}.
-
-Instance enum_unit : enum unit.
-Proof.
-  refine {| list_up_to _ := [tt] |}.
-  intros.
-  destruct a; simpl; auto.
-Defined.
-
-Arguments enum_ty {B} {n}.
-Arguments is_enum_ty {B} {n}.
-
-Fixpoint apply_all_1 {A n} (l : list (enum_component_1 A n)) : list A :=
-  match l with
-  | [] => []
-  | c::cs =>
-      let list_le_n_c := @list_le_n _ _ _ (is_enum_ty c) in
-      apply_1 (constr _ n c) list_le_n_c ++
-                     apply_all_1 cs
-  end.
-
-
-(* Fixpoint apply_all_2 {A n} (l : list (enum_component_2 A n)) : list A := *)
-(*   match l with *)
-(*   | [] => [] *)
-(*   | c::cs => *)
-(*       let list_le_n_c1 := @list_le_n _ _ _ (is_enum_ty1 c) in *)
-(*       let list_le_n_c2 := @list_le_n _ _ _ (is_enum_ty2 c) in *)
-(*       apply_2 (constr _ n c) list_le_n_c1 list_le_n_c2 ++ *)
-(*                      apply_all_2 cs *)
-(*   end. *)
-
-
-(* Instance has_depth_enum_component_1 {A n} : forall (c : enum_component_1 A n), has_depth c. *)
-(* Proof. *)
-(*   intro c; destruct c; auto. *)
-(* Defined. *)
-
-Instance has_depth_enum_componant {A n} : forall (c : enum_component_1 A n), has_depth (enum_ty c).
-Proof.
-  intros c; destruct c; auto.
-Defined.
-
-(* Instance has_depth_enum_component_1 {A n} : forall (c : enum_component_2 A n), has_depth (enum_ty1 c). *)
-(* Proof. *)
-(*   intro c; destruct c; auto. *)
-(* Defined. *)
-
-(* Instance has_depth_enum_component_2 {A n} : forall (c : enum_component_2 A n), has_depth (enum_ty2 c). *)
-(* Proof. *)
-(*   intro c; destruct c; auto. *)
-(* Defined. *)
-
-Lemma all_of_depth_n : forall A n
-                              (h : has_depth A)
-                              (l : list (enum_component_1 A n)),
-    (forall a, depth a <= S n ->
-               exists (c : enum_component_1 A n) (b : enum_ty c),
-                 In c l /\ depth b <= n /\ a = constr _ _ _ b)
-    -> forall a, depth a <= S n -> In a (apply_all_1 l).
-Proof.
-  intros A n h l H a dpth.
-  destruct (H a dpth) as (c & b & mem_l & depth_b & is_cons); subst.
-  clear H dpth.
-  revert c b mem_l depth_b.
-  induction l; simpl; auto.
-  intros c b [h1 | h2] le_b.
-  - apply in_or_app; left.
-    subst; apply mem_apply_1; destruct c.
-    apply is_enum_ty0; auto.
-  - apply in_or_app; right.
-    auto.
-Qed.
-
-
-(* Lemma all_of_depth_n : forall A n *)
-(*                               (h : has_depth A) *)
-(*                               (l1 : list (enum_component_2 A n)), *)
-(*     (forall a, depth a <= S n -> *)
-(*                exists (c : enum_component_2 A n) (b1 : enum_ty1 c)(b2 : enum_ty2 c), *)
-(*                  In c l1 /\ depth b1 <= n /\ depth b2 <= n /\ a = constr _ _ _ b1 b2) *)
-(*     -> forall a, depth a <= S n -> In a (apply_all_2 l1). *)
-(* Proof. *)
-(*   intros. *)
-(*   destruct (H a H0) as (c & b1 & b2 & mem_l1 & depth_b1 & depth_b2 & is_cons); subst. *)
-(*   clear H H0. *)
-(*   revert c b1 b2 mem_l1 depth_b1 depth_b2. *)
-(*   induction l1; simpl; auto. *)
-(*   intros c b1 b2 [h1 | h2] le_b1 le_b2. *)
-(*   - apply in_or_app; left. *)
-(*     subst; apply mem_apply_2; destruct c. *)
-(*     + apply is_enum_ty3; auto. *)
-(*     + apply is_enum_ty4; auto. *)
-(*   - apply in_or_app; right. *)
-(*     auto. *)
-(* Qed. *)
-
-(* Let's define the identity enum_component, since we may need it *)
-Definition id_enum_comp {A} n {d : has_depth A} {e : enum_up_to A n} : enum_component_1 A n :=
-    {|
-      enum_ty := A;
-      constr a := a;
-    |}.
-
-
-Fixpoint depth_tm t :=
-      match t with
-      | var_tm v => S (depth v)
-      | Z => 1
-      | Succ t' => S (depth_tm t')
-      | ha2_syn.Add t1 t2 => S (depth_tm t1 + depth_tm t2)
-      | Mult t1 t2 => S (depth_tm t1 + depth_tm t2)
-      end.
-
-Instance has_depth_tm : has_depth tm :=
-  {| depth := depth_tm |}.
-
-(* We'll bootstrap this later *)
-Instance enum_up_to_tm_0 : enum_up_to tm 0.
-Proof.
-  refine {| list_le_n := [] |}.
-  intros a; destruct a; simpl; lia.
-Defined.
-
-Definition var_tm_enum_comp n : enum_component_1 tm n :=
-    {|
-      enum_ty := fin;
-      constr b := var_tm b;
-    |}.
-
-Definition Z_enum_comp n : enum_component_1 tm n :=
-  {|
-    enum_ty := unit;
-    constr a := Z;
-  |}.
-
-Definition Succ_enum_comp n (h : enum_up_to tm n) : enum_component_1 tm n :=
-  {|
-    enum_ty := tm;
-    constr b := Succ b;
-  |}.
-
-
-(* A bit of proof duplication unfortunately *)
-Instance enum_up_to_pair {A B} n `(ea : enum_up_to A n) `(eb : enum_up_to B n) :
-  enum_up_to (A * B) n.
-Proof.
-  refine {| list_le_n := apply_2 pair list_le_n list_le_n |}.
-  intros [a b] h.
-  destruct ea, eb.
-  simpl in h.
-  apply mem_apply_2; [apply list_has_all_n0; lia | apply list_has_all_n1; lia].
-Defined.
-
-(* Low but should suffice... *)
-Set Typeclasses Depth 10.
-
-Definition Add_enum_comp n (h : enum_up_to tm n) : enum_component_1 tm n :=
-  {|
-    enum_ty := tm * tm;
-    constr (p : tm * tm) := let (a, b) := p in ha2_syn.Add a b;
-  |}.
-
-Definition Mult_enum_comp n (h : enum_up_to tm n) : enum_component_1 tm n :=
-  {|
-    enum_ty := tm * tm;
-    constr p := let (a, b) := p in Mult a b;
-  |}.
-
-
-Check (apply_all_1 ([(var_tm_enum_comp 0); (var_tm_enum_comp 0)])).
-
-Definition incr_enum_tm_fun n (h : enum_up_to tm n) : list tm :=
-  (apply_all_1
-     (
-       [(var_tm_enum_comp n);
-        (* id_enum_comp n; *)(* I thought we'd need this... *)
-        Z_enum_comp n;
-        Succ_enum_comp n _ ;
-        Add_enum_comp n _ ;
-        Mult_enum_comp n _
-       ]
-  )).
-
-Instance incr_enum_tm_enum_up_to n (h : enum_up_to tm n) : enum_up_to tm (S n).
+Instance enum_proof_bundle : enum proof_bundle.
 Proof.
   refine
     {|
-      list_le_n := incr_enum_tm_fun n h
+      list_up_to n :=
+      let props : list prop := list_up_to n in
+      let ctxts : list ctxt := list_up_to n in
+      let pairs := list_prod props ctxts in
+      concat_map (fun '(pair P Γ) =>
+                    let prfs := list_up_to (A := Γ ⊢ P) n in
+                    map (fun p => {| hyps := Γ; concl := P; proof := p |}) prfs)
+                 pairs
     |}.
-  apply all_of_depth_n; auto.
-  destruct a; simpl; intros.
-  - exists (var_tm_enum_comp n).
-    simpl; exists n0; split; auto.
-    repeat split; lia.
-  - exists (Z_enum_comp n).
-    simpl. exists tt.
-    split; auto.
-    repeat split; lia.
-  - exists (Succ_enum_comp n h).
-    simpl; exists a; split; auto.
-    repeat split; lia.
-  - exists (Add_enum_comp n h).
-    simpl. exists (pair a1 a2); split; auto.
-    repeat split; lia.
-  - exists (Mult_enum_comp n h).
-    simpl. exists (pair a1 a2); split; [auto | repeat split; lia].
-    do 4 right; left; auto.
-Defined.
-    
-
-Fixpoint enum_up_to_tm_rec n : enum_up_to tm n :=
-  match n with
-  | 0 => enum_up_to_tm_0
-  | S n' => incr_enum_tm_enum_up_to _ (enum_up_to_tm_rec n')
-  end.
-
-Instance enum_up_to_tm : forall n, enum_up_to tm n :=
-  fun n => enum_up_to_tm_rec n.
-
-(* Nice! *)
-Eval lazy in (@list_le_n tm _ _ (enum_up_to_tm 2)).
-
-Instance enum_tm : enum tm := _.
-
-(* Ok let's see if we can do propositions *)
-
-Fixpoint depth_prop p :=
-  match p with
-  | v ∈ pr => S (depth v + depth_pred pr)
-  | all p' => S (depth_prop p')
-  | FORALL p' => S (depth_prop p')
-  | p1 ⇒ p2 => S (depth_prop p1 + depth_prop p2)
-  end with depth_pred pr :=
-    match pr with
-    | var_pred v => S (depth v)
-    | {{ _ | p }} => S (depth_prop p)
-    end.
-
-Instance has_depth_prop : has_depth prop := {| depth := depth_prop |}.
-Instance has_depth_pred : has_depth pred := {| depth := depth_pred |}.
-
-Instance enum_up_to_prop_0 : enum_up_to prop 0.
-Proof.
-  refine {| list_le_n := [] |}.
-  intros a; destruct a; simpl; lia.
+  intros n a dpth; destruct a.
+  apply in_concat_map.
+  assert (dpth_concl : depth concl0 <= n) by (simpl in dpth; simpl; lia).
+  assert (dpth_hyps : depth hyps0 <= n) by (simpl in dpth; simpl; lia).
+  assert (dpth_proof : depth proof0 <= n) by (simpl in dpth; simpl; lia).
+  clear dpth.
+  exists (pair concl0 hyps0); split.
+  - apply in_prod; apply list_has_all; auto.
+  - apply in_map.
+    apply list_has_all; auto.
 Defined.
 
-
-Instance enum_up_to_pred_0 : enum_up_to pred 0.
-Proof.
-  refine {| list_le_n := [] |}.
-  intros a; destruct a; simpl; lia.
-Defined.
-
-Definition var_pred_enum_comp n : enum_component_1 pred n.
-Proof.
-  refine {| enum_ty := fin |}.
-  exact (fun n => var_pred n).
-Defined.
-
-Definition Mem_prop_enum_comp n
-           (h_pred : enum_up_to pred n)
-  : enum_component_1 prop n.
-Proof.
-  refine {| enum_ty := tm * pred |}.
-  exact (fun '(pair t p) => t ∈ p).
-Defined.
-
-Definition Forallt_prop_enum_comp n
-           (h_prop : enum_up_to prop n)
-  : enum_component_1 prop n.
-Proof.
-  refine {| enum_ty := prop |}.
-  exact (fun p => all p).
-Defined.
-
-Definition Forallp_prop_enum_comp n
-           (h_prop : enum_up_to prop n)
-  : enum_component_1 prop n.
-Proof.
-  refine {| enum_ty := prop |}.
-  exact (fun p => FORALL p).
-Defined.
-
-Definition Impl_prop_enum_comp n
-           (h_prop : enum_up_to prop n)
-  : enum_component_1 prop n.
-Proof.
-  refine {| enum_ty := prop * prop |}.
-  exact (fun '(pair p q) => p ⇒ q).
-Defined.
-
-Definition Comp_pred_enum_comp n
-           (h_prop : enum_up_to prop n)
-  : enum_component_1 pred n.
-Proof.
-  refine {| enum_ty := prop |}.
-  exact (fun p => {{ _ | p }}).
-Defined.
-
-Definition incr_enum_prop_fun (n : fin) (h1 : enum_up_to prop n) (h2 : enum_up_to pred n) : list prop :=
-  apply_all_1
-    ([
-        Mem_prop_enum_comp n h2;
-        Forallt_prop_enum_comp n h1;
-        Forallp_prop_enum_comp n h1;
-        Impl_prop_enum_comp n h1
-    ]).
-
-
-Definition incr_enum_pred_fun (n : fin) (h1 : enum_up_to prop n) (h2 : enum_up_to pred n) : list pred :=
-  apply_all_1
-    ([
-        var_pred_enum_comp n;
-        Comp_pred_enum_comp n h1
-    ]).
-
-Instance incr_enum_prop_enum_up_to n (h1 : enum_up_to prop n)(h2 : enum_up_to pred n) : enum_up_to prop (S n).
-Proof.
-  refine
-    {|
-      list_le_n := incr_enum_prop_fun n h1 h2
-    |}.
-  apply all_of_depth_n; auto.
-  destruct a; simpl; intros.
-  - exists (Mem_prop_enum_comp _ _); simpl.
-    exists (pair t p).
-    intuition; lia.
-  - exists (Forallt_prop_enum_comp _ _); simpl.
-    exists a.
-    intuition.
-  - exists (Forallp_prop_enum_comp _ _); simpl.
-    exists a.
-    intuition.
-  - exists (Impl_prop_enum_comp _ _); simpl.
-    exists (pair a1 a2); intuition; lia.
-Defined.
-
-Instance incr_enum_pred_enum_up_to n (h1 : enum_up_to prop n)(h2 : enum_up_to pred n) : enum_up_to pred (S n).
-Proof.
-  refine
-    {|
-      list_le_n := incr_enum_pred_fun n h1 h2
-    |}.
-  apply all_of_depth_n; auto.
-  destruct a; simpl; intros.
-  - exists (var_pred_enum_comp _); simpl.
-    exists n0; intuition.
-  - exists (Comp_pred_enum_comp _ _); simpl.
-    exists p; intuition.
-Defined.
-
-Fixpoint enum_up_to_prop_rec n : enum_up_to prop n :=
-  match n with
-  | 0 => enum_up_to_prop_0
-  | S n' => incr_enum_prop_enum_up_to
-              n'
-              (enum_up_to_prop_rec n')
-              (enum_up_to_pred_rec n')
-  end
-with enum_up_to_pred_rec n : enum_up_to pred n :=
-       match n with
-       | 0 => enum_up_to_pred_0
-       | S n' => incr_enum_pred_enum_up_to
-                   n'
-                   (enum_up_to_prop_rec n')
-                   (enum_up_to_pred_rec n')
-  end.
-             
-Instance enum_up_to_prop : forall n, enum_up_to prop n :=
-  fun n => enum_up_to_prop_rec n.
-
-Instance enum_up_to_pred : forall n, enum_up_to pred n :=
-  fun n => enum_up_to_pred_rec n.
-
-Instance enum_prop : enum prop := _.
-
-Instance enum_pred : enum pred := _.
-
-(* Ok now proofs! *)
-
-
-Instance has_depth_list {A} {d : has_depth A} : has_depth (list A) :=
-  {|
-    depth := depth_list
-  |}.
-
-Lemma depth_list_len : forall A (d : has_depth A) (l : list A),
-    length l <= depth l.
-Proof.
-  induction l; simpl; auto.
-  unfold depth, has_depth_list in IHl.
-  lia.
-Qed.
-
-Lemma depth_list_In : forall A (d : has_depth A) (l : list A) a,
-    In a l -> depth a <= depth l.
-Proof.
-  intros A d l; induction l; simpl; intros ? h.
-  - contradiction.
-  - destruct h.
-    + subst; lia.
-    + assert (h := IHl _ H).
-      rewrite h.
-      unfold depth; simpl.
-      lia.
-Qed.
-
-Fixpoint cons_all {A} (l : list A) (ll : list (list A)) : list (list A) :=
-  match l with
-  | [] => []
-  | x :: xs => map (fun l' => x :: l') ll ++ cons_all xs ll
-  end.
-
-
-Lemma in_cons_all : forall A (l : list A) (ll : list (list A)) x xs,
-    In x l -> In xs ll -> In (x :: xs) (cons_all l ll).
-Proof.
-  intros A l; induction l; simpl; auto.
-  intros ll x xs.
-  rewrite in_app_iff.
-  intros [hd | tl]; subst.
-  - intros mem; left.
-    revert xs mem.
-    induction ll; simpl; auto.
-    intros xs [h1 | h2]; subst; auto.
-  - auto.
-Qed.
-
-Fixpoint enum_list_len {A} {d : has_depth A} {e : enum A}
-         (len : nat) (dpth : nat) : list (list A) :=
-  match len with
-  | 0 => [[]]
-  | S len' =>
-      let xs : list A := list_up_to dpth in
-      let rec := enum_list_len len' dpth in
-      rec ++ (cons_all xs rec)
-  end.
-
-
-Lemma enum_list_list_in : forall A (d : has_depth A) (e : enum A) l m n,
-    depth l <= n -> length l <= m -> In l (enum_list_len m n).
-Proof.
-  intros A d e l m; revert l.
-  induction m; simpl;
-    intros l; assert (h := depth_list_len _ _ l).
-  - intros; 
-      assert (len_l_zero : length l = 0) by lia.
-    left; symmetry; apply length_zero_iff_nil; auto.
-  - intros n depth_l.
-    rewrite PeanoNat.Nat.le_succ_r.
-    rewrite in_app_iff.
-    intros [h1 | h2].
-    + left; auto.
-    + right.
-      destruct l; [simpl in *; lia | ].
-      simpl in depth_l.
-      apply in_cons_all.
-      -- apply list_has_all; lia.
-      -- simpl in h2;
-           unfold depth in IHm; simpl in IHm;
-           apply IHm; lia.
-Qed.
-      
-
-Definition enum_list {A} {d : has_depth A} {e : enum A} : enum (list A).
-Proof.
-  refine {| list_up_to n := enum_list_len n n |}.
-  intros; apply enum_list_list_in; auto.
-  rewrite (depth_list_len A d) ; auto.
-Defined.
-
-Eval vm_compute in (@enum_list_len fin _ _ 3 3).
-
-Fixpoint depth_derives {Γ P} (d : Γ ⊢ P) : nat :=
-  match d with
-  | axiom n Γ P _ => S (depth Γ)
-  | imp_intro Γ P Q p => S (depth Γ + depth P + depth Q + depth_derives p)
-  | forallt_intro Γ P p => S (depth (lift_tm Γ) + depth P + depth_derives p)
-  | forallP_intro Γ P p => S (depth (lift_prop Γ) + depth P + depth_derives p)
-  | imp_elim Γ P Q p q => S (depth Γ + depth P + depth Q + depth_derives p + depth_derives q)
-  | forallt_elim Γ P t p => S (depth Γ + depth P + depth t + depth_derives p)
-  | forallP_elim Γ P Q p => S (depth Γ + depth P + depth Q + depth_derives p)
-  | compr_intro Γ P t p =>
-      S (depth Γ + depth (subst2 (t .: ids) ids P) + depth_derives p)
-  | compr_elim Γ P t p => S (depth Γ + depth (t ∈ {{_ | P}}) + depth_derives p)
-  | _ => S (depth Γ)
-  end.
-
-Record proof_bundle :=
-  {
-    hyps : ctxt;
-    concl : prop;
-    proof : hyps ⊢ concl;
-  }.
-
-Instance has_depth_proof_bundle : has_depth proof_bundle :=
-  {| depth b := depth (hyps b) + depth (concl b) + depth_derives (proof b) |}.
-
-(* Now just gotta prove that we can enumerate those puppies.*)
-
-Instance enum_up_to_derives_0 : enum_up_to proof_bundle 0.
-Proof.
-  refine {| list_le_n := [] |}.
-  destruct a; simpl.
-  destruct proof0; simpl; lia.
-Defined.
-
-(* Opaque dummy proof, to handle "impossible" cases in our enumeration *)
-Definition dummy_proof : proof_bundle.
-  refine
-    (let h := [var_tm 0 ∈ var_pred 0] in
-     let c := var_tm 0 ∈ var_pred 0 in
-     {|
-       hyps := h;
-       concl := c;
-       proof := axiom 0 h c Logic.eq_refl
-     |}).
-Qed.
-
-
-(* Check (fin * ctxt * prop)%type. *)
-
-Search ({ _ < _} + { _ }).
-About Nat.ltb.
-
-Instance enum_up_to_ctxt n : enum_up_to ctxt n.
-Proof.
-  apply @enum_enum_up_to; apply @enum_list; apply _.
-Defined.
-
-Definition axiom_enum_component n : enum_component_1 proof_bundle n.
-Proof.
-  refine
-    {|
-      enum_ty := fin * ctxt;
-      constr '(pair n Γ) :=
-      if Compare_dec.lt_dec n (length Γ) then _ else dummy_proof
-    |}.
-  econstructor.
-  apply (axiom n).
-  apply nth_error_nth' with (d := (var_tm 0 ∈ var_pred 0)).
-  exact l.
-Defined.
-
-Definition imp_intro_enum_component n (h: enum_up_to proof_bundle n) : enum_component_1 proof_bundle n.
-Proof.
-  refine
-    {|
-      enum_ty := proof_bundle;
-      constr pr :=
-      let '{| hyps := hyps; concl := concl; proof := proof |} := pr in
-      (match hyps as h return hyps = h -> proof_bundle with
-       | [] => fun _ => dummy_proof
-       | P::Ps =>
-           fun _ =>
-             let new_proof := imp_intro _ _ _ _ in
-             {| hyps := Ps; concl := P ⇒ concl; proof := new_proof |}
-       end) (Logic.eq_refl)
-    |}.
-  rewrite<- e.
-  apply proof.
-Defined.
-
-Record has_shape {A B : Type}(unshape : B -> A) :=
-  {
-    shape : A -> option B;
-    shape_correct :
-    forall a b, shape a = Some b <-> unshape b = a
-  }.
+Locate "∃".
 
 
 Definition lower : fin -> fin := Nat.pred.
 
-Require Import ha2.
-
-Definition lower_tm (Γ : ctxt) := map (fun P => P⟨lower; id⟩) Γ.
-Definition lower_prop (Γ : ctxt) := map (fun P => P⟨id; lower⟩) Γ.
-
-Require Import Classes.EquivDec.
-
-
-Lemma dec_prop_eq : forall (p q : prop), {p = q} + {p <> q}
-with dec_pred_eq : forall (p q : pred), {p = q} + {p <> q}.
+Definition lower_prop (P : prop) := P⟨id; lower⟩.
+Lemma lower_lift_prop : forall P, lower_prop (P⟨id; ↑⟩) = P.
 Proof.
-  repeat decide equality.
-  repeat decide equality.
-Defined.
-
-Instance eqdec_prop : EqDec prop eq.
-Proof.
-  exact dec_prop_eq.
-Defined.
-
-Instance eqdec_ctxt : EqDec ctxt eq.
-Proof.
-  apply _.
-Defined.
-
-Lemma lower_lift_tm : forall Γ, lower_tm (lift_tm Γ) = Γ.
-Proof.
-  induction Γ; simpl; auto.
-  asimpl.
-  rewrite IHΓ; f_equal; auto.
+  intros; unfold lower_prop; asimpl.
   erewrite extRen_prop.
   - rewrite rinstId_prop.
     reflexivity.
@@ -746,507 +607,99 @@ Proof.
   - auto.
 Qed.
 
+Locate "∃".
 
-Lemma lower_lift_prop : forall Γ, lower_prop (lift_prop Γ) = Γ.
-Proof.
-  induction Γ; simpl; auto.
-  asimpl.
-  rewrite IHΓ; f_equal; auto.
-  erewrite extRen_prop.
-  - rewrite rinstId_prop.
-    reflexivity.
-  - auto.
-  - auto.
-Qed.
+Print sig.
 
-
-Search (sumbool).
-
-Search (EqDec).
-
-Print equiv_decb.
-
-Print sigT.
-Search sig.
-
-Definition bool_of_sumbool {A B} (o : {A} + {B}) : bool := proj1_sig (Sumbool.bool_of_sumbool o).
-
-Definition has_shape_lift_tm : has_shape lift_tm.
-Proof.
-  refine {| shape Γ :=
-           if lift_tm (lower_tm Γ) ==b Γ then Some (lower_tm Γ) else None
-         |}.
-  intros; split.
-  - unfold "==b".
-    destruct (lift_tm (lower_tm a) == a).
-    + intros h; inversion h.
-      subst; auto.
-    + intros h; inversion h.
-  - intros h; subst.
-    rewrite lower_lift_tm.
-    unfold "==b".
-    destruct (lift_tm b == lift_tm b); auto.
-    destruct c; auto.
-    reflexivity.
+Definition exists_dec (P : prop) : option {Q | P = ∃ Q}.
+  refine
+    (match P with
+     | (FORALL (all Q ⇒ all var_tm 0 ∈ var_pred 0) ⇒ all var_tm 0 ∈ var_pred 0) =>
+         if eqdec_prop ((lower_prop Q)⟨id; ↑⟩) Q then
+           Datatypes.Some (exist _ (lower_prop Q) _)
+         else None
+     | _ => Datatypes.None
+     end).
+  rewrite e; auto.
 Defined.
 
-Definition has_shape_lift_prop : has_shape lift_prop.
-Proof.
-  refine {| shape Γ :=
-           if lift_prop (lower_prop Γ) ==b Γ then Some (lower_prop Γ) else None
-         |}.
-  unfold "==b".
-  intros; split.
-  - destruct (lift_prop (lower_prop a) == a).
-    + intros h; inversion h.
+Require Import ConstructiveEpsilon.
+Section extract.
+
+  Parameter is_dec : prop -> bool.
+
+  Definition ex_val P n := eval_prop bot_pval (n, bot_vval) P.
+  
+  Hypothesis is_dec_correct :
+    forall P,
+      is_dec P ->
+              forall n, { ex_val P n } + { ~ ex_val P n }.
+
+  Definition num_of_proof Γ P (p : Γ ⊢ P) : nat.
+    destruct Γ; [ |  exact 0].
+    destruct (exists_dec P) as [ [Q h] | ]; [|exact 0].
+    destruct (Sumbool.sumbool_of_bool (is_dec Q)) as [dec |]; [| exact 0].
+    eapply constructive_ground_epsilon_nat.
+    - apply is_dec_correct; apply dec.
+    - apply ex_refl.
       subst; auto.
-    + intros h; inversion h.
-  - intros h; subst.
+  Defined.
+
+  Print num_of_proof.
+
+  Theorem num_of_proof_correct : forall P (p : nil ⊢ ∃ P),
+      is_dec P ->
+      ex_val P (num_of_proof nil (∃ P) p).
+  Proof.
+    intros; simpl.
     rewrite lower_lift_prop.
-    destruct (lift_prop b == lift_prop b); auto.
-    destruct c; auto.
-    reflexivity.
-Defined.
+    elim_eqdec.
+    destruct (Sumbool.sumbool_of_bool (is_dec P)); [ | congruence].
+    (* No need to check anything here, it's all in the term! *)
+    apply constructive_ground_epsilon_spec_nat.
+  Qed.
 
-Definition forallt_intro_enum_component n (h: enum_up_to proof_bundle n) : enum_component_1 proof_bundle n.
-Proof.
-  refine
-    {|
-      enum_ty := proof_bundle;
-      constr pr :=
-      let '{| hyps := hyps; concl := concl; proof := proof |} := pr in
-      let hyps_shape := has_shape_lift_tm in
-      let lift_hyps := shape lift_tm hyps_shape hyps in
-      _
-    |}.
-  destruct hyps_shape.
-  simpl in lift_hyps.
-  destruct lift_hyps as [lift_hyps' |] eqn:eq; [ |  exact dummy_proof].
-  econstructor; apply forallt_intro.
-  assert (shape_correct0 := shape_correct0 hyps lift_hyps').
-  assert (shape_correct : shape0 hyps = Some lift_hyps' -> lift_tm lift_hyps' = hyps) by (apply shape_correct0).
-  rewrite shape_correct; auto.
-  exact proof.
-Defined.
+  Definition num_of_all_proofs n : nat :=
+    let proofs : list proof_bundle := list_up_to n in
+    let nums := map (fun '{| hyps := hyps; concl := concl; proof := proof |} =>
+                       num_of_proof hyps concl proof)
+                    proofs
+    in
+    list_max nums.
 
-
-
-Definition forallP_intro_enum_component n (h : enum_up_to proof_bundle n) : enum_component_1 proof_bundle n.
-Proof.
-  refine
-    {|
-      enum_ty := proof_bundle;
-      constr pr :=
-      let '{| hyps := hyps; concl := concl; proof := proof |} := pr in
-      let hyps_shape := has_shape_lift_prop in
-      let lift_hyps := shape lift_prop hyps_shape hyps in
-      _
-    |}.
-  destruct hyps_shape.
-  simpl in lift_hyps.
-  case_eq lift_hyps; intros lift_hyps'; [ |  exact dummy_proof].
-  intros eq; econstructor; apply forallP_intro.
-  subst lift_hyps.
-  rewrite shape_correct0 in eq.
-  subst.
-  apply proof.
-Defined.
-
-Definition has_shape_impl : has_shape (fun '(pair P Q) => P ⇒ Q).
-Proof.
-  refine
-    {|
-      shape P :=
-      match P with
-      | P ⇒ Q => Some (pair P Q)
-      | _ => None
-      end
-    |}.
-  intros a b; destruct a; destruct b; split; intros h; try inversion h; try congruence.
-Defined.
-
-Definition imp_elim_enum_component n (h : enum_up_to proof_bundle n) : enum_component_1 proof_bundle n.
-Proof.
-  refine
-    {|
-      enum_ty := proof_bundle * proof_bundle;
-      constr '(pair pr1 pr2) :=
-      let '{| hyps := hyps1; concl := concl1; proof := proof1 |} := pr1 in
-      let '{| hyps := hyps2; concl := concl2; proof := proof2 |} := pr2 in
-      let concl_shape := has_shape_impl in
-      let arr_concl := shape _ concl_shape concl1 in
-      _
-    |}.
-  destruct concl_shape.
-  simpl in *.
-  case_eq arr_concl; [intros (P & Q) eq | intros; apply dummy_proof ].
-  subst arr_concl.
-  rewrite shape_correct0 in eq.
-  destruct (hyps1 == hyps2); [ | apply dummy_proof].
-  destruct (concl2 == P); [ | apply dummy_proof].
-  subst.
-  econstructor; eapply imp_elim.
-  - apply proof1.
-  - rewrite e.
-    rewrite <- e0.
-    apply proof2.
-Defined.
-
-Print derives.
-
-
-Definition forallt_elim_enum_component n (h : enum_up_to proof_bundle n) : enum_component_1 proof_bundle n.
-Proof.
-  refine
-    {|
-      enum_ty := proof_bundle * tm;
-      constr '(pair pr t) :=
-      let '{| hyps := hyps; concl := concl; proof := proof |} := pr in
-      match concl as c return concl = c -> proof_bundle with
-      | all P => _
-      | _ => fun _ => dummy_proof
-      end  (Logic.eq_refl)
-    |} .
-  intros eq; econstructor.
-  apply forallt_elim.
-  rewrite eq in proof.
-  apply proof.
-  Unshelve.
-  apply Z.
-Defined.
-
-
-Definition forallP_elim_enum_component n (h : enum_up_to proof_bundle n) : enum_component_1 proof_bundle n.
-Proof.
-  refine
-    {|
-      enum_ty := proof_bundle * pred;
-      constr '(pair pr p) :=
-      let '{| hyps := hyps; concl := concl; proof := proof |} := pr in
-      match concl as c return concl = c -> proof_bundle with
-      | FORALL P => _
-      | _ => fun _ => dummy_proof
-      end  (Logic.eq_refl)
-    |} .
-  intros eq; econstructor.
-  apply forallP_elim.
-  rewrite eq in proof.
-  apply proof.
-  Unshelve.
-  apply (var_pred 0).
-Defined.
-
-Print derives.
-
-Print has_shape.
-
-Definition has_shape_tm_subst (P : prop) (t : tm) : has_shape (fun tt : unit => P[t..;ids]).
-Proof.
-  refine {| shape := fun a => if a == P[t..;ids] then Some tt else None |}.
-  intros a [].
-  destruct (a == P[t..; ids]).
-  - rewrite e; intuition.
-  - split; intros h; try congruence.
-    inversion h.
-Defined.
-
-
-Definition compr_intro_enum_component n (h : enum_up_to proof_bundle n) : enum_component_1 proof_bundle n.
-Proof.
-  refine
-    {|
-      enum_ty := proof_bundle * prop * tm;
-      constr '(pair (pair pr p) t) :=
-      let '{| hyps := hyps; concl := concl; proof := proof |} := pr in
-      _
-    |}.
-  pose (shape_p_t := (has_shape_tm_subst p t)).
-  destruct shape_p_t.
-  case_eq (shape0 concl).
-  - intros tt eq.
-    econstructor.
-    apply compr_intro.
-    assert (h': p[t..;ids] = concl) by (eapply shape_correct0; eauto).
-    rewrite<- h' in proof.
-    apply proof.
-  - intros _; exact dummy_proof.
-Defined.
-
-Print derives.
-
-Definition has_shape_mem_compr (P : prop) (t : tm) : has_shape (fun tt : unit => t ∈ {{ _ | P }}).
-Proof.
-  refine {| shape := fun a => if a == t ∈ {{ _ | P }} then Some tt else None |}.
-  intros a [].
-  destruct (a == t ∈ {{ _ | P }}).
-  - rewrite e; intuition.
-  - split; intros h; try congruence.
-    inversion h.
-Defined.
-
-Definition compr_elim_enum_component n (h : enum_up_to proof_bundle n) : enum_component_1 proof_bundle n.
-Proof.
-  refine
-    {|
-      enum_ty := proof_bundle * prop * tm;
-      constr '(pair (pair pr p) t) :=
-      let '{| hyps := hyps; concl := concl; proof := proof |} := pr in
-      _
-    |}.
-  pose (shape_p_t := (has_shape_mem_compr p t)).
-  destruct shape_p_t.
-  case_eq (shape0 concl).
-  - intros tt eq.
-    econstructor.
-    Check compr_elim.
-    Print pred.
-    apply compr_elim.
-    assert (h': (t ∈ {{ _ | p }}) = concl) by (eapply shape_correct0; eauto).
-    rewrite<- h' in proof.
-    apply proof.
-  - intros _; exact dummy_proof.
-Defined.
-
-Print derives.
-
-(* Ugh this is tedious. I should have put axioms into a list or something... *)
-Definition zero_S_enum_component n : enum_component_1 proof_bundle n.
-Proof.
-  refine
-    {|
-      enum_ty := ctxt;
-      constr Γ := {| hyps := Γ; concl := all Succ (var_tm 0) ≄ Z; proof := zero_S Γ |}
-    |}.
-Defined.
-
-Definition inj_S_enum_component n : enum_component_1 proof_bundle n.
-Proof.
-  refine
-    {|
-      enum_ty := ctxt;
-      constr Γ := {| hyps := Γ; concl := all (all Succ (var_tm 1) ≃ Succ (var_tm 0) ⇒ var_tm 1 ≃ var_tm 0); proof := inj_S Γ |}
-    |}.
-Defined.
-
-Definition plus_Z_enum_component n : enum_component_1 proof_bundle n.
-Proof.
-  refine
-    {|
-      enum_ty := ctxt;
-      constr Γ := {| hyps := Γ; concl := all Add (var_tm 0) Z ≃ var_tm 0; proof := plus_Z Γ |}
-    |}.
-Defined.
-
-Definition plus_S_enum_component n : enum_component_1 proof_bundle n.
-Proof.
-  refine
-    {|
-      enum_ty := ctxt;
-      constr Γ := {| hyps := Γ; concl := all (all Add (var_tm 1) (Succ (var_tm 0)) ≃ Succ (Add (var_tm 1) (var_tm 0))); proof := plus_S Γ |}
-    |}.
-Defined.
-
-Definition times_Z_enum_component n : enum_component_1 proof_bundle n.
-Proof.
-  refine
-    {|
-      enum_ty := ctxt;
-      constr Γ := {| hyps := Γ; concl := all Mult (var_tm 0) Z ≃ Z; proof := times_Z Γ |}
-    |}.
-Defined.
-
-Definition times_S_enum_component n : enum_component_1 proof_bundle n.
-Proof.
-  refine
-    {|
-      enum_ty := ctxt;
-      constr Γ := {| hyps := Γ; concl := all (all Mult (var_tm 1) (Succ (var_tm 0)) ≃ Add (var_tm 1) (Mult (var_tm 1) (var_tm 0))); proof := times_S Γ |}
-    |}.
-Defined.
-
-Check incr_enum_pred_enum_up_to.
-
-Print enum_up_to.
-
-Print incr_enum_pred_fun.
-Check apply_all_1.
-Print derives.
-
-Definition incr_enum_proof_bundle_fun n (h : enum_up_to proof_bundle n) :=
-  apply_all_1
-    ([
-        axiom_enum_component n;
-        imp_intro_enum_component n h;
-        forallt_intro_enum_component n h;
-        forallP_intro_enum_component n h;
-        imp_elim_enum_component n h;
-        forallt_elim_enum_component n h;
-        forallP_elim_enum_component n h;
-        compr_intro_enum_component n h;
-        compr_elim_enum_component n h;
-        zero_S_enum_component n;
-        inj_S_enum_component n;
-        plus_Z_enum_component n;
-        plus_S_enum_component n;
-        times_Z_enum_component n;
-        times_S_enum_component n
-    ]).
-
-Check EqDec.
-Lemma EqDec_prop : forall A, EqDec A eq -> forall (a b : A), a = b \/ a <> b.
-Proof.
-  intros A eq a b; destruct (eq a b).
-  - rewrite e; auto.
-  - right; auto.
-Qed.
-
-Require Import Eqdep_dec.
-
-Definition transport_1 {A} {a1 a2} (F : A -> Type) : a1 = a2 -> F a2 -> F a1.
-Proof.
-  intros e; rewrite e; exact (fun x => x).
-Defined.
-
-Definition transport_2 {A B} {a1 a2 : A}{b1 b2 :  B} (F : A -> B -> Type) : a1 = a2 -> b1 = b2 -> F a2 b2 -> F a1 b1.
-Proof.
-  intros e1 e2; rewrite e1; rewrite e2; exact (fun x => x).
-Defined.
-
-Lemma transport_2_refl_l : forall {A B} {a : A}{b1 b2 :  B} (F : A -> B -> Type) (eq: b1 = b2) (x : F a b2), transport_2 F Logic.eq_refl eq x = transport_1 (fun b => F a b) eq x.
-Proof.
-  reflexivity.
-Qed.
-
-Definition eq_bundle (b1 b2 : proof_bundle) :=
-  exists (ph : hyps b1 = hyps b2)(pc : concl b1 = concl b2), (proof b1 = transport_2 (fun a b => a ⊢ b) ph pc (proof b2)).
-
-Theorem eq_bundle_eq : forall b1 b2, eq_bundle b1 b2 -> b1 = b2.
-Proof.
-  destruct b1; destruct b2.
-  unfold eq_bundle; intros (eq1 & eq2 & eq3).
-  simpl in *.
-  rewrite eq3.
-  destruct eq1.
-  destruct eq2.
-  unfold transport_2.
-  unfold eq_rect_r.
-  simpl.
-  reflexivity.
-Qed.
-
-
-Lemma eq_axiom : forall n Γ P Q e1 e2 (eqpq : P = Q),
-    axiom n Γ P e1 = transport_1 _ eqpq (axiom n Γ Q e2).
-Proof.
-  intros until eqpq.
-  destruct eqpq.
-  unfold transport_1, eq_rect_r; simpl.
-  f_equal.
-  apply eq_proofs_unicity.
-  decide equality.
-  apply EqDec_prop; apply _.
-Qed.
-
-Search (_ = left _).
-
-Lemma eq_dec_refl `{EqDec A eq} : forall (x : A), (x == x) = left Logic.eq_refl.
-Proof.
-  intros x.
-  destruct (x == x) as [ |  c]; [f_equal | destruct c; reflexivity ].
-  pattern e at 1.
-  apply K_dec; auto.
-  intros a b; destruct (H a b); auto.
-Qed.
-
-Lemma eqb_refl `{EqDec A eq} : forall (x : A), (x ==b x) = true.
-Proof.
-  intros x; unfold "==b"; destruct (x == x); [ now auto |].
-  destruct c; reflexivity.
-Qed.
-
-Instance eq_dec_ctxt : EqDec ctxt eq := ltac:(apply _).
-
-
-Definition incr_enum_proof_bundle_enum_up_to n (h : enum_up_to proof_bundle n) : enum_up_to proof_bundle (S n).
-Proof.
-  refine
-    {|
-      list_le_n := incr_enum_proof_bundle_fun n h
-    |}.
-  apply all_of_depth_n; simpl; auto.
-  (* This is going to sting *)
-  intros a; remember a as bndl.
-  destruct a as [hyps concl proof].
-  destruct proof; intros.
-  - subst; simpl in *.
-    exists (axiom_enum_component n).
-    exists (pair n0 Γ).
-    split; [simpl; left; now auto | ].
-    split; simpl.
-    + simpl in *.
-      assert (n0 <= depth_list Γ).
-      {
-        assert (n0 < length Γ) by (apply nth_error_Some; destruct (nth_error Γ n0); auto; inversion e; try congruence).
-        assert (len_depth := depth_list_len _ _ Γ); simpl in *.
+  Lemma list_max_ge : forall l m,
+      (exists n, In n l /\ m <= n) -> m <= list_max l.
+  Proof.
+    intros l m [n [in_n m_le_n]].
+    induction l; simpl.
+    - destruct in_n.
+    - simpl in in_n.
+      destruct in_n.
+      + subst.
         lia.
-      }
-      lia.
-    + destruct (Compare_dec.lt_dec n0 (length Γ));
-        [ |
-          clear H;
-          assert (n0 < length Γ);
-          try apply nth_error_Some;
-          try (intros e'; rewrite e' in e; inversion e);
-          contradiction].
-      apply eq_bundle_eq.
-      assert (e' : P = nth n0 Γ (var_tm 0 ∈ var_pred 0)) by (symmetry; apply nth_error_nth; auto).
-      exists Logic.eq_refl, e'.
-      rewrite transport_2_refl_l.
-      simpl.
-      apply eq_axiom.
-  - exists (imp_intro_enum_component n h).
-    exists {| hyps := P :: Γ; concl := Q; proof := proof0 |}.
-    split; [right; left; now auto | ].
-    split; [ | subst; simpl; now auto].
-    subst.
-    simpl in *.
-    lia.
-  - exists (forallt_intro_enum_component n h).
-    exists {| hyps := lift_tm Γ; concl := P; proof := proof0 |}.
-    split; [right; right; left; now auto |].
-    split.
-    + simpl.
-      subst; simpl in *.
-      lia.
-    + subst.
-      clear H.
-      simpl.
-      rewrite lower_lift_tm.
-      rewrite eqb_refl.
-      Search (_ ==b _).
-      
-      dependent destruction (lift_tm (lower_tm (lift_tm Γ)) ==b lift_tm Γ).
-      pattern (if @equiv_decb _ eq _ eqdec_ctxt (lift_tm (lower_tm (lift_tm Γ))) (lift_tm Γ)
-               then Some (lower_tm (lift_tm Γ))
-               else None).
+      + assert (h := IHl H).
+        lia.
+  Qed.
+    
+  Print has_depth_proof_bundle.
+  Eval compute in depth nil.
 
-      replace (if @equiv_decb _ eq _ eqdec_ctxt (lift_tm (lower_tm (lift_tm Γ))) (lift_tm Γ)
-               then Some (lower_tm (lift_tm Γ))
-               else None)
-        with (Some (lower_tm (lift_tm Γ))).
+  Theorem num_of_all_proofs_lt : forall m P (p : nil ⊢ (∃ P)),
+      is_dec P ->
+      (forall n, ex_val P n -> m <= n) ->
+      m <= num_of_all_proofs ((depth (∃ P)) + (depth p)).
+  Proof.
+    intros m P p dec ex.
+    unfold num_of_all_proofs.
+    apply list_max_ge.
+    exists (num_of_proof nil (∃ P) p).
+    split; [ | apply ex; apply num_of_proof_correct; now auto].
+    Search (In _ (list_map _ _)).
+    apply in_map_iff.
+    exists {| hyps := nil; concl := (∃ P); proof := p |}.
+    split; [ now auto |].
+    apply list_has_all.
+    reflexivity.
+Qed.  
 
-
-      pattern (lift_tm (lower_tm (lift_tm Γ)) ==b lift_tm Γ) at 2.
-      
-      (* replace (lift_tm (lower_tm (lift_tm Γ))) with (lift_tm Γ). *)
-      (* rewrite lower_lift_tm. *)
-      (* pose (my_case := *)
-      (*         (if lift_tm (lower_tm (lift_tm Γ)) == lift_tm Γ *)
-      (*          then Some (lower_tm (lift_tm Γ)) *)
-      (*          else None)). *)
-      (* assert (my_case = Some Γ). *)
-      (* { unfold my_case. *)
-      (*   rewrite lower_lift_tm. *)
-      (*   rewrite eq_dec_refl; auto. *)
-      (* }. *)
-      (* unfold my_case in H0; rewrite H0. *)
+End extract.
